\section{Refined Strings}\label{sec:strings}

Refined Strings provides a wrapping over a string manipulations library, 
here `ByteString`
\begin{code}
data RString = S BS.ByteString 
\end{code}

String operators wrap the library operators
and moreover they are assumed to be reflected into the logic

\begin{code}
assume concatString :: x:LHString -> y:LHString 
      -> {v:LHString | v == concatString x y }
concatString (S s1) (S s2) = S (s1 `BS.append` s2)

assume stringEmp :: {v:RString | v == stringEmp  && stringLen v == 0 } 
stringEmp = S (BS.empty)

assume stringLen :: x:RString -> {v:Nat | v == stringLen x}
stringLen (S s) = BS.length s 

assume subString  :: s:RString -> offset:Int -> ln:Int -> {v:RString | v == subString s offset ln }
subString (S s) o l = S (BS.take l (BS.drop o s))

assume takeString :: i:Nat -> xs:{RString | i <= stringLen xs } 
  -> {v:RString | stringLen v == i && v == takeString i xs }
takeString i (S s) = S (BS.take i s)

assume dropString :: i:Nat -> xs:{RString | i <= stringLen xs } 
  -> {v:RString | stringLen v == stringLen xs - i && v == dropString i xs }
dropString i (S s) = S (BS.drop i s)

assume fromString :: i:String -> {o:RString | i == o && o == fromString i}
fromString = S . ST.fromString 

assume isNullString :: i:RString -> {b:Bool | Prop b <=> stringLen i == 0 }
isNullString (S s) = BS.length s == 0 
\end{code}


Finally the refined string library, exposes theorems that hold (but are assumed) 
for the internal string representation

\begin{code}
assume stringEmpProp :: x:RString  -> { stringLen x == 0 <=> x == stringEmp }
stringEmpProp _ = trivial 
 
assume concatStringNeutralLeft :: x:RString -> {concatString x stringEmp == x}
concatStringNeutralLeft _ = trivial

assume concatStringNeutralRight :: x:RString -> {concatString stringEmp x == x}
concatStringNeutralRight _ = trivial

assume concatTakeDrop :: i:Nat -> xs:{RString | i <= stringLen xs} 
    -> {xs == concatString (takeString i xs) (dropString i xs) }
concatTakeDrop _ _ = trivial

assume concatLen :: x:RString -> y:RString -> { stringLen (concatString x y) == stringLen x + stringLen y }
concatLen _ _ = trivial

assume concatStringAssoc :: x:RString -> y:RString -> z:RString 
     -> {concatString (concatString x y) z == concatString x (concatString y z) }
concatStringAssoc _ _ _ = trivial


-- | Substrings 

assume subStringConcatBack :: input:RString -> input':RString -> j:Int -> i:{Int | i + j <= stringLen input }
  -> { (subString input i j == subString (concatString input input') i j) }
subStringConcatBack _ _ _ _ = trivial  


assume subStringConcatFront  
  :: input:RString -> input':RString -> j:Int -> i:Int 
  -> { (subString input i j == subString (concatString input' input) (stringLen input' + i) j) }
subStringConcatFront _ _ _ _ = trivial
\end{code}