Assume \hastype{\emptyset}{e}{\tau}.
We will prove the Lemma by induction on the derivation tree.
\begin{itemize}
\item Case \rtvar cannot occur, as $\Gamma = \emptyset$
\item Case \rtbot is trivial, 
		as $\lnot \botomless{e}$.
\item Cases \rtconst and \rtfun are trivial, 
		as $e = v$.
\item Case \rtsub. Assume \hastype{\emptyset}{e}{\tau}.
By inversion
$$	\hastype{\emptyset}{e}{\tau'}$$
By IH 
either $e \equiv v$ or there exists an botomless $e'$ such that \eval{e}{e'}.
\item Case \rtapp. Assume $$\hastype{\emptyset}{e}{\tau}\ (1)$$
where $e\equiv\eapp{e_1}{e_2}$ and $\tau\equiv\tau'\sub{x}{e_2}$.
By inversion
$$
	\hastype{\emptyset}{e_1}{(\tfun{x}{\tau_{x}}{\tau})}\ (2)\qquad
	\hastype{\emptyset}{e_2}{\tau_{x}}\ (3)
$$

We split cases on the structure of $e$.
\begin{itemize}
\item $e\equiv \eapp{c}{v_2}$.
Then, $e'\equiv\interp{c}(v_2)$ which is botomless by Definition of constants.

\item $e\equiv \eapp{c}{e_2}$ where $e_2$ is not a value, 
By IH on $(3)$ \eval{e_2}{e_2'} and  $e' \equiv \eapp{e_1}{e_2'}$

\item $e \equiv \eapp{\efun{x}{e_x}}{e_2}$.
Then, $e' \equiv e_x\sub{x}{e_2}$, which does not contain bottom.

\item $e \equiv \eapp{e_1}{e_2}$, where $e_1 \neq v$.
Then, by IH on $(2)$ \eval{e_1}{e_1'} and 
$e'\equiv\eapp{e_1'}{e_2}$.
\end{itemize}

\item Case \rtlet. Assume \hastype{\emptyset}{e}{\tau}, where 
$e \equiv \elet{x}{e_x}{e_0}$, then $e'\equiv e_0\sub{x}{e_x}$ which is botomless.

\item Case \rtcase. Assume \hastype{\emptyset}{e}{\tau}, where
$e \equiv \ecase{e_T}{D_{T_i}}{\overline{y}}{e_i}{x}$.
By inversion, 
$$
	\hastype{\Gamma}{e}{\tref{v}{T}{e_T}}\ (1)
$$
We split cases on the structure of $e_T$
\begin{itemize}
\item If $e_T$ is a value, then by $(1)$ it is of the form $e_T \equiv D_{T_i} \overline{e}$,
so $e' \equiv e_i \sub{x}{e_T}\overline{\sub{y}{e}} $
\item Otherwise, by IH there exists $e'_T$ such that \evals{e_T}{e'_T}, 
so $e' \equiv \ecase{e'_T}{D_{T_i}}{\overline{y}}{e_i}{x}$.
\end{itemize}
\end{itemize}