\section{Reasoning About Lambdas}\label{sec:lambdas}

Soundness and precision of \corelan relies 
on the $\beta$-equivalence and extensionality axioms that are undecidable. 
%
Next, we present a decidable but incomplete way 
to approximate $\beta$-equivalence
by strengthening the VCs with equalities~\S~\ref{subsec:equivalences},
and extensionality by introducing a combinator for safely asserting
extensional equality~\S~\ref{subsec:extensionality}.
%
In the rest of this section, 
for clarity we omit $\smtappname{}{}$ when it is clear from the context.

\subsection{Equivalence}\label{subsec:equivalences}

As soundness relies on axioms of $\beta$-equivalence
we can safely \emph{instantiate} the axioms of
$\alpha$- and $\beta$-equivalence on any set of
terms of our choosing and still preserve soundness.
%
That is, instead of checking the validity
of a VC
${p \Rightarrow q}$,
we check the validity of a \emph{strengthened VC},
${a \Rightarrow p \Rightarrow q}$,
where $a$ is a (finite) conjunction
of \emph{equivalence instances}
derived from $p$ and $q$,
as discussed below.

% Since it is unclear how to reify this axiomatization
% while preserving decidability, we choose (once again)
% to syntactically instantiate the axioms of $\alpha$-,
% $\beta$- and normal form equivalence on the relevant
% candidates.

\mypara{Representation Invariant}
%
The lambda binders,
for each SMT sort, are drawn from a
pool of names $x_i$ where the index
$i=1,2,\ldots$.
%
When representing
$\lambda$ terms we enforce
a \emph{normalization invariant}
that for each lambda term
$\slam{x_i}{e}$, the index $i$
% $x_i$
is greater than any lambda
argument appearing in $e$.

\mypara{$\alpha$-instances}
For each syntactic term
${\slam{x_i}{e}}$, and $\lambda$-binder
$x_j$ such that $i < j$ appearing in the VC,
we generate an \emph{$\alpha$-equivalence instance predicate}
(or \emph{$\alpha$-instance}):
$$\slam{x_i}{e} = \slam{x_j}{e \subst{x_i}{x_j}}$$

% , x_i < x_j \leq \maxlamarg$$
%\leq \maxlamarg$
% that follow the ordering
% $i < j \Leftrightarrow x_i < x_j$.
%
% The number of distinct valid lambda
% arguments is determined by the
% maximum number of $\lambda$s
% syntactically in program's refinements.
% In the implementation, we bound
% this number by $\maxlamarg = 7$.
% %
% In practice we only encountered
% 4 nested lambdas when verifying
% monadic left identity of the
% reader monad.

The conjunction of $\alpha$-instances
can be more precise than De Bruijn
representation, as they let the SMT
solver deduce more equalities via
congruence.
%
For example, consider the VC needed
to prove the applicative laws for @Reader@:
%
\begin{align*}
d  = \slam{x_1}{(\sapp{x}{x_1})} 
   \Rightarrow \slam{x_2}{(\sapp{(\slam{x_1}{(\sapp{x}{x_1})})}{x_2})}
              = \slam{x_1}{(\sapp{d}{x_1})}
\end{align*}
%
The $\alpha$ instance
%
${\slam{x_1}{(\sapp{d}{x_1})} = \slam{x_2}{(\sapp{d}{x_2})}}$
%
derived from the VC's hypothesis,
combined with congruence immediately
yields the VC's consequence.

\mypara{$\beta$-instances}
%
For each syntactic term $\smapp{(\slam{x}{e})}{e_x}$,
with $e_x$ not containing any $\lambda$-abstractions,
appearing in the VC,
we generate an \emph{$\beta$-equivalence instance predicate}
(or \emph{$\beta$-instance}):
$$
\smapp{(\slam{x_i}{e})}{e_x} = \SUBST{e}{x_i}{e_x},
  \mbox{ s.t. } e_x \mbox{ is $\lambda$-free}
$$
%
We require the $\lambda$-free restriction as
a simple way to enforce that the reduced
term ${\SUBST{e}{x_i}{e'}}$ enjoys the
representation invariant.
%
%%\NV{This restriction is not implemented, but neither has a normalization function}
%%\RJ{Then why are we discussing it?}

For example, consider the following VC
needed to prove that the bind operator for
lists satisfies the monadic associativity law.
%
$$(\sapp{f}{x} \ebind g) = \smapp{(\slam{y}{(\sapp{f}{y} \ebind g)})}{x}$$
%
The right-hand side of the above VC generates
a $\beta$-instance that corresponds directly
to the equality, allowing the SMT solver to
prove the (strengthened) VC.

%% immediately yields
%% $\beta$-equivalence is required in our benchmarks to for example prove
%% monadic associativity for lists.
%% %
%% An intermediate step in the proof is to verify that
%%
%% Assuming that @h x = f x >>= g@ the above
%% translates to the logical query
%% $$
%% \sapp{h}{x} = \sapp{(\slam{x_1}{(\sapp{h}{x_1})})}{x}
%% $$
%%
%% The right hand side of the query will fire a
%% $\beta$-equivalence instantiation
%% and the assumption
%% $
%% \sapp{(\slam{x_1}{(\sapp{h}{x_1})})}{x} = \sapp{h}{x}
%% $
%% will be added in the environment, allowing SMT to prove the equivalence.

\mypara{Normalization}
%
The combination of $\alpha$- and $\beta$-instances
is often required to discharge proof obligations.
%
For example, when proving that the bind operator
for the @Reader@ monad is associative, we need
to prove the VC:
%
$$\slam{x_2}{(\slam{x_1}{w})} =
  \slam{x_3}{(\smapp{(\slam{x_2}{(\slam{x_1}{w})})}{w})}$$
%
The SMT solver proves the VC via the equalities
corresponding to an $\alpha$ and then $\beta$-instance:
%
\begin{align*}
\slam{x_2}{(\slam{x_1}{w})}
  \ =_{\alpha}\ & \slam{x_3}{(\slam{x_1}{w})} \\
  \ =_{\beta}\ & \slam{x_3}{(\smapp{(\slam{x_2}{(\slam{x_1}{w})})}{w})}
\end{align*}

%%% of monadic
%%% associativity for the reader monad requires to prove a $\lambda$ equality
%%% simplified to
%%% %
%%% \begin{code}
  %%% w:a -> {(\x y -> w) = (\x -> (\z y -> w) w)}
%%% \end{code}
%%% %
%%% The proof for the above code is @trivial@ as
%%% in the logic, the $\lambda$ arguments are renamed to
%%% @(\x2 x1 -> w) = (\x3 -> (\x2 x1 -> w) w)@.
%%% Due to $\alpha$- equivalence the
%%% right hand side is equal to
%%% @\x3 x1 -> w@.
%%% Due to $\beta$-equivalence we get
%%% @((\x2 x1 -> w) w) = \x1 -> w@,
%%% by which and due to congruence axiom
%%% we get the desired equality,
%%% \begin{code}
  %%% \x y -> w               -- lhs
  %%% \x2 x1 -> w             -- representation
  %%% \x3 x1 -> w             -- alpha
  %%% \x3 ->((\x2 x1 -> w) w) -- beta
  %%% \x -> ((\z y -> w) w)   -- rhs
%%% \end{code}

\subsection{Extensionality} \label{subsec:extensionality}

Often, we need to prove that two
functions are equal, given the
definitions of reflected binders.
%
For example, consider
%
\begin{code}
  reflect id
  id x = x
\end{code}
%
\toolname accepts the proof that
@id x = x@ for all @x@:
%
\begin{code}
  id_x_eq_x :: x:a -> {id x = x}
  id_x_eq_x = \x -> #id# x =. x ** QED
\end{code}
%
as ``calling'' @id@ unfolds its definition,
completing the proof.
%
However, consider this $\eta$-expanded variant of
the above proposition:
%
\begin{code}
  type Id_eq_id = {(\x -> id x) = (\y -> y)}
\end{code}
%
\toolname \emph{rejects} the proof:
%
\begin{code}
  fails :: Id_eq_id
  fails =  (\x -> #id# x) =. (\y -> y) ** QED
\end{code}
%
The invocation of @id@ unfolds the
definition, but the resulting equality
refinement @{id x = x}@ is \emph{trapped}
under the $\lambda$-abstraction.
%
That is, the equality is absent from the
typing environment at the \emph{top} level,
where the left-hand side term is compared to @\y -> y@.
%
% NV LHS reads like LiquidHaskell
Note that the above equality requires
the definition of @id@ and hence is
outside the scope of purely the
$\alpha$- and $\beta$-instances.

\newcommand\eqfun{\ensuremath{\texttt{=}\forall}}

\mypara{An Exensionality Operator}
%
To allow function equality via
extensionality, we provide the
user with a (family of)
%
\emph{function comparison operator(s)}
that transform an \emph{explanation} @p@
which is a proof that @f x = g x@ for every
argument @x@, into a proof that @f = g@.
%
\begin{mcode}
  =* :: f:(a -> b) -> g:(a -> b)
     -> exp:(x:a -> {f x = g x})
     -> {f = g}
\end{mcode}
%
Of course, @=*@ cannot be implemented;
its type is \emph{assumed}. We can use
@=*@ to prove @Id_eq_id@ by providing
a suitable explanation:
%
\begin{mcode}
  pf_id_id :: Id_eq_id
  pf_id_id = (\y -> y) =* (\x -> id x) $\because$ expl ** QED
   where
     expl  = (\x -> #id# x =. x ** QED)
\end{mcode}
%
%   =* (\x -> id x) $\because$ exp
%   where
%    exp   :: x:a -> {(\x -> id x) x = (\x -> x) x}
%    exp x = #id# x =. x ** QED
%
The explanation is
% the proof passed as
the second argument to $\because$ which has
the following type that syntactically fires $\beta$-instances:
\begin{code}
  x:a -> {(\x -> id x) x = ((\x -> x) x}
\end{code}

